

PHSX 711: Homework #8

November 21, 2024

Grant Saggars

Problem 1

Exercise 12.2.1 (Shankar) – 5 points

Provide the steps linking Eq. (12.2.8) to Eq. (12.2.9). [Hint: Recall the derivation of Eq. (11.2.8) from Eq. (11.2.6).]

$$\begin{aligned} U[R] |x, y\rangle &= |x - y\epsilon_z, x\epsilon_z + y\rangle \\ \langle x, y| I - \frac{i\epsilon_z L_z}{\hbar} |\psi\rangle &= \psi(x + y\epsilon_z, y - x\epsilon_z) \end{aligned}$$

Solution: In the derivation of rotations, we initially define infinitesimal rotations about $\epsilon_z \mathbf{k}$:

$$U[R(\epsilon_z \mathbf{k})] = I - \frac{i\epsilon_z L_z}{\hbar}$$

We can first examine the hermitian conjugate, where we just end up inverting the sign on the parts multiplied by ϵ_z . Then, we can consider the application of the rotation operator such that $\langle x, y| U[R] |\psi\rangle$ to rotate the coordinates which we project ψ into. This leaves us with a modified projection of ψ onto x' and y' .

$$\begin{aligned} (U[R] |x, y\rangle)^\dagger &= \langle x, y| \left(I + \frac{i\epsilon_z L_z}{\hbar} \right) = \langle x + y\epsilon_z, -x\epsilon_z + y| \\ \langle x, y| I - \frac{i\epsilon_z L_z}{\hbar} |\psi\rangle &= \langle x + y\epsilon_z, -x\epsilon_z + y| \psi\rangle \\ &= \psi(x + y\epsilon_z, y - x\epsilon_z) \end{aligned}$$

Problem 2

Exercise 12.2.3 (Shankar) – 5 points

Derive Eq. (12.2.19) by doing a coordinate transformation on Eq. (12.2.10), and also by the direct method mentioned above.

$$L_z \underset{\text{coordinate basis}}{=} -i\hbar \frac{\partial}{\partial \phi}$$

*You can choose either one of the methods.

Solution:

Equation 12.2.10 says

$$L_z = x \left(-i\hbar \frac{\partial}{\partial y} \right) - y \left(-i\hbar \frac{\partial}{\partial x} \right)$$

Directly doing the coordinate transformation to this is probably more straightforward. The only tricky part is working out the transformation of the partial derivatives to polar coordinates for $r = 1$ (since we don't want to modify length of our vectors).

$$\begin{aligned} &= \cos \phi \left(-i\hbar \frac{\partial}{\partial \phi} \frac{\partial \phi}{\partial y} \right) - \sin \phi \left(-i\hbar \frac{\partial}{\partial \phi} \frac{\partial \phi}{\partial x} \right) \\ &= \cos \phi \left(-i\hbar \cos \phi \frac{\partial}{\partial \phi} \right) - \sin \phi \left(-i\hbar \sin \phi \frac{\partial}{\partial \phi} \right) \\ &= -i\hbar (\cos^2 \phi + \sin^2 \phi) \frac{\partial}{\partial \phi} \\ &= -i\hbar \frac{\partial}{\partial \phi} \end{aligned}$$

Problem 3

Exercise 12.5.3 (Shankar) – 10 points

(1) Show that $\langle J_x \rangle = \langle J_y \rangle = 0$ in a state $|jm\rangle$.

Solution: We have

$$J_i = L_i + S_i$$

Which in the basis of ladder operators is:

$$J_x = \frac{J_+ + J_-}{2}, \quad J_y = \frac{J_+ - J_-}{2i}$$

Which we do know how to do calculations with:

$$J_{\pm} |jm\rangle = \hbar[(j \mp m)(j \pm m + 1)]^{1/2} |j, m \pm 1\rangle$$

It is relatively simple to express expectation values:

$$\begin{aligned}
 \langle jm | \frac{J_+ + J_-}{2} | jm \rangle &= \frac{1}{2} [\langle jm | J_+ | jm \rangle + \langle jm | J_- | jm \rangle] \\
 &= \frac{\hbar}{2} \left\{ [(j-m)(j+m+1)]^{1/2} \langle jm | j, m+1 \rangle + [(j+m)(j-m+1)]^{1/2} \langle jm | j, m-1 \rangle \right\}^0 \\
 &= 0 \\
 \langle jm | \frac{J_+ - J_-}{2i} | jm \rangle &= \frac{1}{2i} [\langle jm | J_+ | jm \rangle - \langle jm | J_- | jm \rangle] \\
 &= \frac{\hbar}{2i} \left\{ [(j-m)(j+m+1)]^{1/2} \langle jm | j, m+1 \rangle - [(j+m)(j-m+1)]^{1/2} \langle jm | j, m-1 \rangle \right\}^0 \\
 &= 0
 \end{aligned}$$

We run into the same situation we do with harmonic oscillator ladder operators, in that our off-diagonal (block diagonal) matrix form results in expectation values of zero when a value gets raised but not lowered, and vice versa due to the delta function.

(2) Show that in these states

$$\langle J_x^2 \rangle = \langle J_y^2 \rangle = \frac{1}{2} \hbar^2 [j(j+1) - m^2]$$

(use symmetry arguments to relate $\langle J_x^2 \rangle$ to $\langle J_y^2 \rangle$).

Solution: As with the harmonic oscillator ladder operators, squaring the sum of these operators results in two terms that have equal amounts raising and lowering.

$$\begin{aligned}
 \frac{1}{2} \langle jm | (J_+ + J_-)^2 | jm \rangle &= \frac{1}{2} \langle jm | J_+^2 + J_-^2 + J_- J_+ + J_+ J_- | jm \rangle \\
 -\frac{1}{2} \langle jm | (J_+ - J_-)^2 | jm \rangle &= \frac{1}{2} \langle jm | J_+^2 - J_-^2 - J_- J_+ + J_+ J_- | jm \rangle
 \end{aligned}$$

Where the sequence of the one lowering-raising operator and vice-versa is:

$$\begin{aligned}
 \langle jm | J_- J_+ | jm \rangle &= \hbar [(j-m)(j+m+1)]^{1/2} \langle jm | J_- | jm+1 \rangle \\
 &= \hbar^2 [(j-m)(j+m+1)(j+(m+1))(j-(m+1)+1)]^{1/2} \langle jm | j, m \rangle^1 \\
 &= \hbar^2 (j+m+1)(j-m) \\
 \langle jm | J_+ J_- | jm \rangle &= \hbar [(j+m)(j-m+1)]^{1/2} \langle jm | J_+ | jm-1 \rangle \\
 &= \hbar^2 [(j+m)(j-m+1)(j-(m-1))(j+(m-1)+1)]^{1/2} \langle jm | j, m \rangle^1 \\
 &= \hbar^2 (j+m)(j-m+1)
 \end{aligned}$$

Substituting these back in,

$$\langle J_x^2 \rangle = \frac{1}{2} \langle jm | (J_+ + J_-)^2 | jm \rangle = \frac{\hbar^2}{2} [(j+m+1)(j-m) + (j+m)(j-m+1)] = \frac{\hbar^2}{2} [j(j+1) - m^2]$$

It happens that $\langle J_y^2 \rangle$ is the same, since that extra i in the demoninator when squared makes it identical to $\langle J_x^2 \rangle$.

Solution #2: A bit more compactly, we have rotational invariance about the z -axis, so $\langle J_x^2 \rangle = \langle J_y^2 \rangle$. Now we can just work out expectation values for:

$$J^2 - J_z^2 = J_x^2 + J_y^2$$

which is the same:

$$\langle J_x^2 \rangle = \langle J_y^2 \rangle = \frac{\hbar^2}{2} [j(j+1) - m^2]$$

(3) Check that $\Delta J_x \cdot \Delta J_y$ from part (2) satisfies the inequality imposed by the uncertainty principle [Eq. (9.2.9)].

Solution: We have equation (9.2.9):

$$(\Delta\Omega)^2(\Delta\Lambda)^2 \geq |\langle \psi | \Omega\Lambda | \psi \rangle|^2$$

where $\Omega\Lambda$ can also be expressed in terms of commutators

$$\frac{[\Omega, \Lambda]_+ + [\Omega, \Lambda]}{2}$$

I think that it will be easier to just directly compute their product, since it is just

$$\langle J_x J_y \rangle = \frac{1}{4i} \langle J_- J_+ - J_+ J_- \rangle = \frac{m\hbar^2}{2}$$

Now the left hand side, we have by rotational invariance about the z -axis:

$$\begin{aligned} \Delta J_x = \Delta J_y &= \sqrt{\langle J_x^2 \rangle - \langle J_x \rangle^2} \\ &= \sqrt{\frac{\hbar^2}{2} [j(j+1) - m^2]} \end{aligned}$$

So to verify, we have

$$\frac{\hbar^2}{2} [j(j+1) - m^2] \geq \frac{m\hbar^2}{2}$$

We must realize that $j \leq |m| \implies j(j+1) \leq m(m+1)$, so then the equality is met.

(4) Show that the uncertainty bound is saturated in the state $|j, \pm j\rangle$.

Solution: The inequality is only saturated when $j = |m| \implies m = \pm j$. This is the state $|j, \pm j\rangle$

Problem 4

Exercise 12.5.12 (Shankar) – 6 points

Since L^2 and L_z commute with Π , they should share a basis with it. Verify that $Y_l^m \xrightarrow{\Pi} Y_{l\Pi}^m = (-1)^l Y_l^m$.

Hint: (I expanded the hint from the book a little bit)

1. $Y_{l\Pi}^m$ in this question represents the function generated from ΠY_l^m .
2. Recall (from Chap. 11) that Π is an operation that changes (x, y, z) to $(-x, -y, -z)$. For spherical coordinates, $\Pi Y_l^m = Y_{l\Pi}^m(\theta, \phi) = Y_l^m(\pi - \theta, \phi + \pi)$
3. Show the proof for the Y_l^l first.
4. Then, show that the lower operator L_- (projected in the X-basis) is not altered by the parity operation $(\theta \rightarrow \pi - \theta, \phi \rightarrow \phi + \pi)$

Solution:

We have the harmonic function

$$Y_l^m(\theta, \phi) = \left[\frac{(2l+1)(l-m)!}{4\pi(l+m)!} \right]^{1/2} (-1)^m e^{im\phi} P_l^m(\cos \theta)$$

Starting with (3), we can apply the parity operator to Y_l^l .

$$Y_l^l(\theta, \phi) = \left[\frac{2l+1}{4\pi(2l)!} \right]^{1/2} (-1)^l e^{il\phi} P_l^l(\cos \theta)$$

$$\Pi Y_l^l(\theta, \phi) = \left[\frac{2l+1}{4\pi(2l)!} \right]^{1/2} (-1)^l e^{il(\phi+\pi)} P_l^l(\cos(\pi - \theta))$$

A key thing to see here is that P_l^l obeys a nice rule, where

$$P_l^l = \sin^l \theta = \sin^l(\pi - \theta)$$

We don't really care about the normalization term since it doesn't change under parity, so under parity just need to know what happens to the exponential ϕ term.

$$e^{il(\phi+\pi)} = (e^{i\phi})^l e^{il\pi} = (-1)^l e^{il\phi}$$

Hence,

$$\Pi Y_l^l = (-1)^l Y_l^l$$

We can now lower the harmonic function using L_- to access the values of $m \neq l$. Recall that the operator L_{\pm} is defined as

$$L_{\pm} = \pm \hbar e^{i\phi} \left(\frac{\partial}{\partial \theta} \pm i \cot \theta \frac{\partial}{\partial \phi} \right).$$

Under the transformations $\theta \rightarrow \pi - \theta$ and $\phi \rightarrow \phi + \pi$, the differentials remain unchanged except that the differential with respect to θ picks up a negative sign.

To verify the behavior of $\cot \theta$ under these transformations, we only need to check whether

$$\cot \theta \stackrel{?}{=} \cot(\pi - \theta),$$

since it was already shown that $e^{i\phi} \rightarrow e^{i(\phi-\pi)} = (-1)^l e^{i\phi}$.

Using trigonometric identities, we compute:

$$\cot(\pi - \theta) = \frac{\cos(\pi - \theta)}{\sin(\pi - \theta)} = \frac{-\cos \theta}{\sin \theta} = -\cot \theta.$$

Thus, $\cot(\pi - \theta) = -\cot \theta$, confirming the behavior of L_- under the transformation.

$$L_- = \Pi L_- \implies [L_-, \Pi] = 0$$

Therefore

$$\Pi Y_l^m = (-1)^l Y_l^m$$

Problem 5

Exercise 12.6.1 (Shankar) – 9 points

A particle is described by the wave function

$$\psi_E(r, \theta, \phi) = A e^{-r/a_0} \quad (a_0 = \text{const})$$

(1) What is the angular momentum content of the state?

Solution: No ϕ or θ dependence implies it has no angular momentum. Furthermore, $\psi_E \propto Y_0^0$.

(2) Assuming ψ_E is an eigenstate in a potential that vanishes as $r \rightarrow \infty$, find E . (Match leading terms in Schrödinger's equation.)

Solution:

$$\begin{aligned} \hat{H}\psi_E &= \left[-\frac{\hbar^2}{2\mu} \frac{1}{r^2} \frac{\partial}{\partial r} \left(r^2 \frac{\partial}{\partial r} \right) + V(r) \right] \psi_E = E\psi_E \\ &\left[-\frac{\hbar^2}{2\mu} \frac{1}{r^2} \frac{\partial}{\partial r} \left(r^2 \frac{\partial}{\partial r} \right) + V(r) \right] A e^{-r/a_0} = E A e^{-r/a_0} \\ &\left[-\frac{\hbar^2}{2\mu} \frac{1}{r^2} \frac{\partial}{\partial r} \left(r^2 \frac{\partial}{\partial r} (A e^{-r/a_0}) \right) + V(r) A e^{-r/a_0} \right] = E A e^{-r/a_0} \\ &-\frac{\hbar^2}{2\mu} \frac{1}{r^2} \frac{A}{a_0^2} (2a_0 r - r^2) e^{-r/a_0} + V(r) A e^{-r/a_0} = E A e^{-r/a_0} \\ &-\frac{\hbar^2}{2\mu} \frac{1}{r^2} \frac{1}{a_0^2} (2a_0 r - r^2) + V(r) = E \\ &-\frac{\hbar^2}{\mu a_0} + \frac{\hbar^2}{2\mu a_0 r} + V(r) = E \end{aligned}$$

If potential vanishes as $r \rightarrow \infty$, then we are left with one term

$$E = -\frac{\hbar^2}{\mu a_0}$$

(3) Having found E , consider finite r and find $V(r)$.

Solution: Substituting E in, we have

$$-\frac{\hbar^2}{2\mu a_0 r} = V(r)$$